Lemma/Tensor/GetKeepdim/as/KeepdimGet/of/Lt_Get_0/Gt_0/Lt_Length.lean
@@ -1,0 +1,26 @@
+import sympy.tensor.functions
+import Lemma.List.Lt_LengthInsertIdxEraseIdx.of.Lt_Length
+import Lemma.Tensor.Length.eq.Get_0.of.GtLength_0
+import Lemma.Tensor.LengthSum.eq.Length.of.Gt_0
+import Lemma.Tensor.Sum.as.Stack_Sum.of.LtAdd_1Length
+import Lemma.Tensor.EqGetS.of.Eq.Lt_Length
+import Lemma.Tensor.EqGetStack.of.Lt
+open Tensor List
+
+
+@[main]
+private lemma main
+  {dim i : ℕ}
+  {s : List ℕ}
+-- given
+  (h : dim < s.length)
+  (h₁ : dim > 0)
+  (h_i : i < s[0])
+  (X : Tensor α (s.eraseIdx dim)) :
+-- imply
+  X.keepdim.get ⟨i, by sorry⟩ ≃ ((X.unsqueeze dim).repeat s[dim] ⟨dim, Lt_LengthInsertIdxEraseIdx.of.Lt_Length h 1⟩).get ⟨i, by sorry⟩ := by
+-- proof
+  sorry
+
+
+-- created on 2025-10-09
