Lemma/Tensor/GetSoftmax/eq/SoftmaxGet/of/Lt_Get_0/Gt_0/Lt_Length.lean
@@ -2,7 +2,9 @@ import sympy.tensor.functions
 import Lemma.Tensor.Length.eq.Get_0.of.GtLength_0
 import Lemma.Tensor.GetDiv.eq.DivGetS
 import Lemma.Tensor.GetExp.eq.ExpGet
-open Tensor
+import Lemma.Tensor.LengthExp.eq.Length
+import Lemma.Bool.EqUFnS.of.Eq
+open Tensor Bool
 
 
 @[main]
@@ -22,9 +24,11 @@ private lemma main
   intro h_i' h_i
   unfold Tensor.softmax
   simp [GetElem.getElem]
-  rw [GetDiv.eq.DivGetS.fin]
-  rw [GetExp.eq.ExpGet.fin]
+  rw [GetDiv.eq.DivGetS.fin (i := ⟨i, by simpa [LengthExp.eq.Length]⟩)]
+  rw [GetExp.eq.ExpGet.fin (i := ⟨i, h_i⟩)]
+  apply EqUFnS.of.Eq _ (exp (X.get ⟨i, h_i⟩) / ·)
   sorry
 
 
 -- created on 2025-10-08
+-- updated on 2025-10-09
