Lemma/Tensor/GetSum/as/SumGet/of/Lt_Get_0/LtAdd_1Length.lean
@@ -1,6 +1,6 @@
 import Lemma.Tensor.Length.eq.Get_0.of.GtLength_0
 import Lemma.Tensor.LengthSum.eq.Length.of.Gt_0
-import Lemma.Tensor.Sum.as.Stack_Sum.of.Add_1.lt.Length
+import Lemma.Tensor.Sum.as.Stack_Sum.of.LtAdd_1Length
 import Lemma.Tensor.EqGetS.of.Eq.Lt_Length
 import Lemma.Tensor.EqGetStack.of.Lt
 open Tensor
@@ -20,7 +20,7 @@ private lemma main
   (X.sum (dim + 1))[i] ≃ X[i].sum dim := by
 -- proof
   intro h_i_length _
-  have := Sum.as.Stack_Sum.of.Add_1.lt.Length h_dim X
+  have := Sum.as.Stack_Sum.of.LtAdd_1Length h_dim X
   have h_i' : i < (X.sum (dim + 1)).length := by
     rwa [LengthSum.eq.Length.of.Gt_0 (by linarith)]
   have := EqGetS.of.Eq.Lt_Length h_i' this
