Lemma/Tensor/Sum/eq/GetEllipsisKeepdimSum/of/Get/gt/Zero.lean
@@ -20,9 +20,10 @@ private lemma main
   (h : s[dim] > 0)
   (X : Tensor α s) :
 -- imply
-  X.sum dim = (X.sum_keepdim dim).getEllipsis dim ⟨0, h⟩ := by
+  X.sum dim = (X.sum dim).keepdim.getEllipsis dim ⟨0, h⟩ := by
 -- proof
-  unfold Tensor.sum_keepdim
+  unfold Tensor.keepdim
+  simp
   have h_lt := LtVal dim
   have h_dim := Lt_LengthInsertIdxEraseIdx.of.Lt_Length h_lt 1
   have h_cast := GetEllipsisCast.eq.Cast_GetEllipsis.of.Eq
